\documentclass[problem]{mcs}

\begin{pcomments}
  \pcomment{CP_sum_of_3i-1_squares_S15}
  \pcomment{by Shen, Elizabeth 2/17/15}
  \pcomment{factoring 6n^3+21n^2+23n+8 = (n+1)(6n^2+15n+8) too cumbersone for an exam}
  \pcomment{format ARM 10/30/15}
\end{pcomments}

\pkeywords{
  induction
  sum
  squares
}
	
%%%%%%%%%%%%%%%%%%%%%%%%%%%%%%%
%PROBLEM STARTS HERE%%%%%%%%%%%
%%%%%%%%%%%%%%%%%%%%%%%%%%%%%%%

\begin{problem}
Prove by induction that for all $n \geq 1$,
\[
 \sum_{i=1}^n (3i-1)^2 = \frac{n(6n^2+3n-1)}{2}
\]
using the equation itself as the induction hypothesis, $P(n)$. 

\bparts

\ppart Prove the \inductioncase{Base case} $(n=1)$.

\begin{solution}
\[
\sum_{i=1}^1 (3i-1)^2 = 4 = \frac{1\cdot 8}{2}.
\]
Therefore, $P(1)$ is true.
\end{solution}

\examspace[1in]

\ppart Now prove the \inductioncase{Inductive step}.

\begin{solution}
\begin{align*}
\sum_{i=1}^{n+1} (3i-1)^2 
& = \paren{\sum_{i=1}^{n} (3i-1)^2} + (3(n+1)-1)^2 \\ 
& = \frac{n(6n^2+3n-1)}{2} + (3n+2)^2 & \text{(by induction hypothesis)}\\
& = \frac{(6n^3+3n^2-n)}{2} + (9n^2+12n+4) \\ 
& = \frac{(6n^3+21n^2+23n+8)}{2}\\
& = \frac{(n+1)(6n^2+15n+8)}{2} \\ 
& = \frac{(n+1)(6(n+1)^2+3(n+1)-1)}{2}.
\end{align*}
Thus we have proved $P(n+1)$, completing the induction step. 
We conclude by induction that $P(n)$ holds for all $n \in \nngint^{+}$.
\end{solution}	

\end{problem}

\endinput
