\documentclass[problem]{mcs}

\begin{pcomments}
  \pcomment{MQ_Summation-morning-alternation}
  \pcomment{same as MQ_Summation-afternoon}
  \pcomment{from TP_Summation}
  \pcomment{Converted from summation.scm
    by scmtotex and dmj
    on Sun 13 Jun 2010 03:24:16 PM EDT}
  \pcomment{revised by drewe on 2 Aug 2011}
\end{pcomments}

\begin{problem}

%% type: multi-part
%% title: Summation

Show that this series converges:
\begin{equation*}
    \sum_{i=1}^\infty (-1)^{i} \frac{1}{i} = -1+\frac{1}{2}-\frac{1}{3}+\frac{1}{4}-\cdots
\end{equation*}
\hint{$\sum_{n=1}^\infty \frac{1}{n^2}$ converges.}


\begin{solution}
\begin{equation*}
\sum_{i=1}^\infty (-1)^{i} \frac{1}{i} = -1+\frac{1}{2}-\frac{1}{3}+\frac{1}{4}+\cdots = -1+\frac{1}{2*3}+\frac{1}{4*5}+\cdots = -1+\sum_{i=1}^\infty \frac{1}{(2i)(2i+1)} < \sum_{i=1}^\infty \frac{1}{(2i)^2} < \sum_{i=1}^\infty \frac{1}{i^2}.
\end{equation*}
\end{solution}

\end{problem}

\endinput
